providers/evercrypt/fst/EverCrypt.Hash.fst
@@ -46,8 +46,8 @@ type state_s: alg -> Type0 =
 | SHA2_256_s: p:Hacl.Hash.Definitions.state SHA2_256 -> state_s SHA2_256
 | SHA2_384_s: p:Hacl.Hash.Definitions.state SHA2_384 -> state_s SHA2_384
 | SHA2_512_s: p:Hacl.Hash.Definitions.state SHA2_512 -> state_s SHA2_512
-| Blake2S_s: p:Hacl.Hash.Definitions.state Blake2S -> counter:extra_state Blake2S -> state_s Blake2S
-| Blake2B_s: p:Hacl.Hash.Definitions.state Blake2B -> counter:extra_state Blake2B -> state_s Blake2B
+| Blake2S_s: p:Hacl.Hash.Definitions.state Blake2S -> state_s Blake2S
+| Blake2B_s: p:Hacl.Hash.Definitions.state Blake2B -> state_s Blake2B
 
 let invert_state_s (a: alg): Lemma
   (requires True)
@@ -56,7 +56,7 @@ let invert_state_s (a: alg): Lemma
 =
   allow_inversion (state_s a)
 
-let mk_state_s (#a:alg) (p:Hacl.Hash.Definitions.state a) (es:extra_state a) :
+let mk_state_s (#a:alg) (p:Hacl.Hash.Definitions.state a) :
   GTot (state_s a) =
   match a with
   | MD5 -> MD5_s p
@@ -65,8 +65,8 @@ let mk_state_s (#a:alg) (p:Hacl.Hash.Definitions.state a) (es:extra_state a) :
   | SHA2_256 -> SHA2_256_s p
   | SHA2_384 -> SHA2_384_s p
   | SHA2_512 -> SHA2_512_s p
-  | Blake2S -> Blake2S_s p es
-  | Blake2B -> Blake2B_s p es
+  | Blake2S -> Blake2S_s p
+  | Blake2B -> Blake2B_s p
 
 inline_for_extraction
 let p #a (s: state_s a): Hacl.Hash.Definitions.state a =
@@ -77,8 +77,8 @@ let p #a (s: state_s a): Hacl.Hash.Definitions.state a =
   | SHA2_256_s p -> p
   | SHA2_384_s p -> p
   | SHA2_512_s p -> p
-  | Blake2S_s p _ -> p
-  | Blake2B_s p _ -> p
+  | Blake2S_s p -> p
+  | Blake2B_s p -> p
 
 let freeable_s #a s = B.freeable (p #a s)
 
@@ -88,15 +88,9 @@ let footprint_s #a (s: state_s a) =
 let invariant_s #a (s: state_s a) h =
   B.live h (p s)
 
-let extra_state_s (#a:alg) (s: state_s a) : extra_state a =
-  match s with
-  | Blake2S_s _ ev -> ev
-  | Blake2B_s _ ev -> ev
-  | _ -> ()
-
 let repr #a s h: GTot _ =
   let s = B.get h s 0 in
-  as_seq h (p s), extra_state_s s
+  as_seq h (p s)
 
 let alg_of_state a s =
   let open LowStar.BufferOps in
@@ -107,11 +101,11 @@ let alg_of_state a s =
   | SHA2_256_s _ -> SHA2_256
   | SHA2_384_s _ -> SHA2_384
   | SHA2_512_s _ -> SHA2_512
-  | Blake2S_s _ _ -> Blake2S
-  | Blake2B_s _ _ -> Blake2B
+  | Blake2S_s _ -> Blake2S
+  | Blake2B_s _ -> Blake2B
 
-let repr_eq (#a:alg) (r1 r2: Spec.Hash.Definitions.words_state a) =
-  Seq.equal (fst r1) (fst r2) /\ snd r1 == snd r2
+let repr_eq (#a:alg) (r1 r2: Spec.Hash.Definitions.words_state' a) =
+  Seq.equal r1 r2
 
 let fresh_is_disjoint l1 l2 h0 h1 = ()
 
@@ -119,7 +113,7 @@ let invariant_loc_in_footprint #a s m = ()
 
 let frame_invariant #a l s h0 h1 =
   let state = B.deref h0 s in
-  assert (repr_eq (repr s h0) (repr s h1))
+  assert (repr_eq #a (repr #a s h0) (repr #a s h1))
 
 inline_for_extraction noextract
 let alloca a =
@@ -131,8 +125,8 @@ let alloca a =
     | SHA2_256 -> SHA2_256_s (B.alloca 0ul 8ul)
     | SHA2_384 -> SHA2_384_s (B.alloca 0UL 8ul)
     | SHA2_512 -> SHA2_512_s (B.alloca 0UL 8ul)
-    | Blake2S -> Blake2S_s (B.alloca 0ul 16ul) (nat_to_extra_state Blake2S 0)
-    | Blake2B -> Blake2B_s (B.alloca 0uL 16ul) (nat_to_extra_state Blake2B 0)
+    | Blake2S -> Blake2S_s (B.alloca 0ul 16ul)
+    | Blake2B -> Blake2B_s (B.alloca 0uL 16ul)
   in
   B.alloca s 1ul
 
@@ -145,8 +139,8 @@ let create_in a r =
     | SHA2_256 -> SHA2_256_s (B.malloc r 0ul 8ul)
     | SHA2_384 -> SHA2_384_s (B.malloc r 0UL 8ul)
     | SHA2_512 -> SHA2_512_s (B.malloc r 0UL 8ul)
-    | Blake2S -> Blake2S_s (B.malloc r 0ul 16ul) (nat_to_extra_state Blake2S 0)
-    | Blake2B -> Blake2B_s (B.malloc r 0uL 16ul) (nat_to_extra_state Blake2B 0)
+    | Blake2S -> Blake2S_s (B.malloc r 0ul 16ul)
+    | Blake2B -> Blake2B_s (B.malloc r 0uL 16ul)
   in
   B.malloc r s 1ul
 
@@ -163,8 +157,8 @@ let init #a s =
   | SHA2_256_s p -> Hacl.Hash.SHA2.init_256 p
   | SHA2_384_s p -> Hacl.Hash.SHA2.init_384 p
   | SHA2_512_s p -> Hacl.Hash.SHA2.init_512 p
-  | Blake2S_s p _ -> let ev = Hacl.Hash.Blake2.init_blake2s p in s *= Blake2S_s p ev
-  | Blake2B_s p _ -> let ev = Hacl.Hash.Blake2.init_blake2b p in s *= Blake2B_s p ev
+  | Blake2S_s p -> let ev = Hacl.Hash.Blake2.init_blake2s p in s *= Blake2S_s p
+  | Blake2B_s p -> let ev = Hacl.Hash.Blake2.init_blake2b p in s *= Blake2B_s p
 #pop-options
 
 friend Vale.SHA.SHA_helpers
@@ -200,7 +194,7 @@ let update_multi_224 s ev blocks n =
 
 // Need to unroll the definition of update_multi once to prove that it's update
 #push-options "--max_fuel 1 --ifuel 1"
-let update #a s block =
+let update #a s prevlen block =
   match !*s with
   | MD5_s p -> Hacl.Hash.MD5.legacy_update p () block
   | SHA1_s p -> Hacl.Hash.SHA1.legacy_update p () block
@@ -208,17 +202,18 @@ let update #a s block =
   | SHA2_256_s p -> update_multi_256 p () block 1ul
   | SHA2_384_s p -> Hacl.Hash.SHA2.update_384 p () block
   | SHA2_512_s p -> Hacl.Hash.SHA2.update_512 p () block
-  | Blake2S_s p ev ->
-      let ev = Hacl.Hash.Blake2.update_blake2s p ev block in
-      s *= Blake2S_s p ev
-  | Blake2B_s p ev ->
-      let ev = Hacl.Hash.Blake2.update_blake2b p ev block in
-      s *= Blake2B_s p ev
+  | Blake2S_s p ->
+      let ev' = Hacl.Hash.Blake2.update_blake2s p prevlen block in
+      s *= Blake2S_s p
+  | Blake2B_s p ->
+      [@inline_let] let prevlen = Int.Cast.Full.uint64_to_uint128 prevlen in
+      let ev' = Hacl.Hash.Blake2.update_blake2b p prevlen block in
+      s *= Blake2B_s p
 #pop-options
 
 #push-options "--ifuel 1"
 
-let update_multi #a s blocks len =
+let update_multi #a s prevlen blocks len =
   match !*s with
   | MD5_s p ->
       let n = len / block_len MD5 in
@@ -238,14 +233,15 @@ let update_multi #a s blocks len =
   | SHA2_512_s p ->
       let n = len / block_len SHA2_512 in
       Hacl.Hash.SHA2.update_multi_512 p () blocks n
-  | Blake2S_s p ev ->
+  | Blake2S_s p ->
       let n = len / block_len Blake2S in
-      let ev = Hacl.Hash.Blake2.update_multi_blake2s p ev blocks n in
-      s *= Blake2S_s p ev
-  | Blake2B_s p ev ->
+      let ev = Hacl.Hash.Blake2.update_multi_blake2s p prevlen blocks n in
+      s *= Blake2S_s p
+  | Blake2B_s p ->
+      [@inline_let] let prevlen = Int.Cast.Full.uint64_to_uint128 prevlen in
       let n = len / block_len Blake2B in
-      let ev = Hacl.Hash.Blake2.update_multi_blake2b p ev blocks n in
-      s *= Blake2B_s p ev
+      let ev = Hacl.Hash.Blake2.update_multi_blake2b p prevlen blocks n in
+      s *= Blake2B_s p
 
 #pop-options
 
@@ -319,7 +315,7 @@ let update_last_128 a update_last p ev prev_len last last_len =
 let update_last_with_internal_st (a : alg) =
   s:state a ->
   p:Hacl.Hash.Definitions.state a ->
-  es:extra_state a ->
+//  es:extra_state a ->
   prev_len:uint64_t ->
   last:B.buffer Lib.IntTypes.uint8 { B.length last <= block_length a } ->
   last_len:uint32_t {
@@ -330,15 +326,15 @@ let update_last_with_internal_st (a : alg) =
   Stack unit
   (requires fun h0 ->
     invariant s h0 /\
-    B.get h0 s 0 == mk_state_s p es /\
+    B.get h0 s 0 == mk_state_s p /\
     B.live h0 last /\
     M.(loc_disjoint (footprint s h0) (loc_buffer last) /\
-    extra_state_v (snd (repr s h0)) + v last_len <= max_input_length a))
+    v prev_len + v last_len <= max_input_length a))
   (ensures fun h0 _ h1 ->
     invariant s h1 /\
     repr s h1 ==
-      Spec.Hash.Incremental.update_last a (repr s h0) (v prev_len)
-                                        (B.as_seq h0 last) /\
+      fst (Spec.Hash.Incremental.update_last a (repr_with_counter s h0 prev_len) (v prev_len)
+                                             (B.as_seq h0 last)) /\
     M.(modifies (footprint s h0) h0 h1) /\
     footprint s h0 == footprint s h1 /\
     preserves_freeable s h0 h1)
@@ -346,35 +342,37 @@ let update_last_with_internal_st (a : alg) =
 inline_for_extraction noextract
 val update_last_blake2s : update_last_with_internal_st Blake2S
 
-let update_last_blake2s s p ev prev_len last last_len =
+let update_last_blake2s s p prev_len last last_len =
   let h0 = ST.get () in
+  [@inline_let] let ev = prev_len in
   let ev' = update_last_64 Blake2S Hacl.Hash.Blake2.update_last_blake2s p ev
                            prev_len last last_len in
-  s *= Blake2S_s p ev';
+  s *= Blake2S_s p;
   let h2 = ST.get () in
-  assert(M.(modifies (footprint s h0) h0 h2));
   assert(
     repr s h2 ==
-      Spec.Hash.Incremental.update_last Blake2S (repr s h0) (v prev_len)
-                                        (B.as_seq h0 last));
-   assert(footprint s h0 == footprint s h2)
+      fst (Spec.Hash.Incremental.update_last Blake2S (repr_with_counter s h0 prev_len)
+                                             (v prev_len) (B.as_seq h0 last)));
+  assert(footprint s h0 == footprint s h2);
+  assert(M.(modifies (footprint s h0) h0 h2))
 
 inline_for_extraction noextract
 val update_last_blake2b : update_last_with_internal_st Blake2B
 
-let update_last_blake2b s p ev prev_len last last_len =
+/// This proof often loops
+let update_last_blake2b s p prev_len last last_len =
   let h0 = ST.get () in
+  [@inline_let] let ev = Int.Cast.Full.uint64_to_uint128 prev_len in
   let ev' = update_last_128 Blake2B Hacl.Hash.Blake2.update_last_blake2b p ev
                             prev_len last last_len in
-  let h1 = ST.get () in
-  s *= Blake2B_s p ev';
+  s *= Blake2B_s p;
   let h2 = ST.get () in
-  assert(M.(modifies (footprint s h0) h0 h2));
   assert(
     repr s h2 ==
-      Spec.Hash.Incremental.update_last Blake2B (repr s h0) (v prev_len)
-                                        (B.as_seq h0 last));
-   assert(footprint s h0 == footprint s h2)
+      fst (Spec.Hash.Incremental.update_last Blake2B (repr_with_counter s h0 prev_len)
+                                             (v prev_len) (B.as_seq h0 last)));
+  assert(footprint s h0 == footprint s h2);
+  assert(M.(modifies (footprint s h0) h0 h2))
 
 let update_last #a s prev_len last last_len =
   match !*s with
@@ -390,10 +388,10 @@ let update_last #a s prev_len last last_len =
       update_last_128 a Hacl.Hash.SHA2.update_last_384 p () prev_len last last_len
   | SHA2_512_s p ->
       update_last_128 a Hacl.Hash.SHA2.update_last_512 p () prev_len last last_len
-  | Blake2S_s p ev ->
-      update_last_blake2s s p ev prev_len last last_len
-  | Blake2B_s p ev ->
-      update_last_blake2b s p ev prev_len last last_len
+  | Blake2S_s p ->
+      update_last_blake2s s p prev_len last last_len
+  | Blake2B_s p ->
+      update_last_blake2b s p prev_len last last_len
 
 #push-options "--ifuel 1"
 
@@ -405,8 +403,8 @@ let finish #a s dst =
   | SHA2_256_s p -> Hacl.Hash.SHA2.finish_256 p () dst
   | SHA2_384_s p -> Hacl.Hash.SHA2.finish_384 p () dst
   | SHA2_512_s p -> Hacl.Hash.SHA2.finish_512 p () dst
-  | Blake2S_s p ev -> Hacl.Hash.Blake2.finish_blake2s p ev dst
-  | Blake2B_s p ev -> Hacl.Hash.Blake2.finish_blake2b p ev dst
+  | Blake2S_s p -> Hacl.Hash.Blake2.finish_blake2s p 0UL dst
+  | Blake2B_s p -> Hacl.Hash.Blake2.finish_blake2b p (UInt128.uint_to_t 0) dst
 
 #pop-options
 
@@ -418,8 +416,8 @@ let free #ea s =
     | SHA2_256_s p -> B.free p
     | SHA2_384_s p -> B.free p
     | SHA2_512_s p -> B.free p
-    | Blake2S_s p _ -> B.free p
-    | Blake2B_s p _ -> B.free p
+    | Blake2S_s p -> B.free p
+    | Blake2B_s p -> B.free p
   end;
   B.free s
 
@@ -457,18 +455,18 @@ let copy #a s_src s_dst =
       let s_dst: state SHA2_512 = s_dst in
       let p_dst = SHA2_512_s?.p !*s_dst in
       B.blit p_src 0ul p_dst 0ul 8ul
-  | Blake2S_s p_src ev_src ->
+  | Blake2S_s p_src ->
       [@inline_let]
       let s_dst: state Blake2S = s_dst in
       let p_dst = Blake2S_s?.p !*s_dst in
       B.blit p_src 0ul p_dst 0ul 16ul;
-      s_dst *= Blake2S_s p_dst ev_src
-  | Blake2B_s p_src ev_src ->
+      s_dst *= Blake2S_s p_dst
+  | Blake2B_s p_src ->
       [@inline_let]
       let s_dst: state Blake2B = s_dst in
       let p_dst = Blake2B_s?.p !*s_dst in
       B.blit p_src 0ul p_dst 0ul 16ul;
-      s_dst *= Blake2B_s p_dst ev_src
+      s_dst *= Blake2B_s p_dst
 
 #pop-options
 
